



**Question.1.** If  $W_1, W_2$  are subspaces of a vector space  $V$ , then

$$\dim(W_1 + W_2) = \dim(W_1) + \dim(W_2) - \dim(W_1 \cap W_2).$$

**Solution:** Let  $W_1, W_2$  be subspaces of a vector space  $V$  and  $S$  be a basis of  $W_1 \cap W_2$  (if  $W_1 \cap W_2$  is the zero space then  $S = \emptyset$ ). For each  $i = 1, 2$ , extend  $S$  to a basis  $B_i$  of  $W_i$ .

Let  $S = \{\mathbf{u}_1, \mathbf{u}_2, \dots, \mathbf{u}_r\}$ ,  $B_1 = \{\mathbf{u}_1, \mathbf{u}_2, \dots, \mathbf{u}_r, \mathbf{v}_1, \mathbf{v}_2, \dots, \mathbf{v}_s\}$ ,  $B_2 = \{\mathbf{u}_1, \mathbf{u}_2, \dots, \mathbf{u}_r, \mathbf{w}_1, \mathbf{w}_2, \dots, \mathbf{w}_t\}$ .

Then  $\dim(W_1) = r + s$ ,  $\dim(W_2) = r + t$ . Let  $B = \{\mathbf{u}_1, \dots, \mathbf{u}_r, \mathbf{v}_1, \dots, \mathbf{v}_s, \mathbf{w}_1, \dots, \mathbf{w}_t\}$ .

It is enough to show that  $B$  is a basis of  $\mathbf{w}_1 + \mathbf{w}_2$  because then

$$\dim(W_1 + W_2) = r + s + t = (r + s) + (r + t) - r = \dim(W_1) + \dim(W_2) - \dim(W_1 \cap W_2)$$

To show that  $B$  is linearly independent, we need to show that

$$\sum_{i=1}^r a_i \mathbf{u}_i + \sum_{j=1}^s b_j \mathbf{v}_j + \sum_{k=1}^t c_k \mathbf{w}_k = \mathbf{0} \quad (1)$$

implies  $a_i = b_j = c_k = 0$  for all  $i, j, k$ . Let (1) be re-expressed as:

$$\sum_{i=1}^r a_i \mathbf{u}_i + \sum_{j=1}^s b_j \mathbf{v}_j = - \sum_{k=1}^t c_k \mathbf{w}_k. \quad (2)$$

Let  $\mathbf{v} \triangleq - \sum_{k=1}^t c_k \mathbf{w}_k$ . Now the LHS of (2) is in  $W_1$  and the RHS is in  $W_2$ . Thus,  $\mathbf{v} \in W_1 \cap W_2$  and  $\mathbf{v} = \sum_{i=1}^r d_i \mathbf{u}_i$  for some scalars  $d_i \in \mathbb{R}$ . Since  $\mathbf{v} = - \sum_{k=1}^t c_k \mathbf{w}_k = \sum_{i=1}^r d_i \mathbf{u}_i$ , it now follows that:

$$\sum_{i=1}^r d_i \mathbf{u}_i + \sum_{k=1}^t c_k \mathbf{w}_k = \mathbf{0},$$

which implies  $d_i = 0$  and  $c_k = 0$  for each  $i, k$  (since  $B_2$  is linearly independent). We can now revise (1) as:

$$\sum_{i=1}^r a_i \mathbf{u}_i + \sum_{j=1}^s b_j \mathbf{v}_j = \mathbf{0},$$

which implies  $a_i = b_j = 0$  for each  $i, j$  (since  $B_1$  is linearly independent). Thus,  $B$  is linearly independent.

Showing that  $W_1 + W_2 = \text{span}(B)$  is rather straightforward; nevertheless, we include the argument here for completeness. Note that the vectors in  $B$  belong to  $W_1 + W_2$ . Since  $W_1 + W_2$  is a vector space, any linear combination of its elements also belongs to it, and hence  $\text{span}(B) \subseteq W_1 + W_2$ . To show that  $W_1 + W_2 \subseteq \text{span}(B)$ , consider any vector  $\mathbf{x} \in W_1 + W_2$ . By definition of  $W_1 + W_2$ , we have  $\mathbf{x} = \mathbf{w}_1 + \mathbf{w}_2$  for some  $\mathbf{w}_1 \in W_1$  &  $\mathbf{w}_2 \in W_2$ . Let  $\mathbf{w}_1 = \sum_{i=1}^r \alpha_i \mathbf{u}_i + \sum_{j=1}^s \beta_j \mathbf{v}_j$  and  $\mathbf{w}_2 = \sum_{i=1}^r \gamma_i \mathbf{u}_i + \sum_{k=1}^t \eta_k \mathbf{w}_k$ . Thus:

$$\begin{aligned} \mathbf{x} = \mathbf{w}_1 + \mathbf{w}_2 &= \left( \sum_{i=1}^r \alpha_i \mathbf{u}_i + \sum_{j=1}^s \beta_j \mathbf{v}_j \right) + \left( \sum_{i=1}^r \gamma_i \mathbf{u}_i + \sum_{k=1}^t \eta_k \mathbf{w}_k \right) \\ \implies \mathbf{x} &= \sum_{i=1}^r (\alpha_i + \gamma_i) \mathbf{u}_i + \sum_{j=1}^s \beta_j \mathbf{v}_j + \sum_{k=1}^t \eta_k \mathbf{w}_k \end{aligned}$$

So, any vector of  $W_1 + W_2$  can be expressed as a linear combination of vectors of  $B$ . Hence,  $B$  is a basis for  $W_1 + W_2$  and this completes the proof.

**Question 2.** Let  $A = \begin{pmatrix} 1 & 0 & 0 \\ 0 & 2 & 0 \\ 0 & 0 & 3 \end{pmatrix}$ . Consider the linear transformation  $\varphi(\mathbf{x}) = A\mathbf{x}$ .

Obtain the transformation matrix with respect to the basis vectors  $\mathcal{B} = \left\{ \begin{pmatrix} 1 \\ 2 \\ 4 \end{pmatrix}, \begin{pmatrix} 0 \\ 1 \\ 0 \end{pmatrix}, \begin{pmatrix} 0 \\ 0 \\ 1 \end{pmatrix} \right\}$ .

**Solution.** Given:

$$\mathcal{B} = \left\{ \mathbf{b}_1 = \begin{pmatrix} 1 \\ 2 \\ 4 \end{pmatrix}, \mathbf{b}_2 = \begin{pmatrix} 0 \\ 1 \\ 0 \end{pmatrix}, \mathbf{b}_3 = \begin{pmatrix} 0 \\ 0 \\ 1 \end{pmatrix} \right\}.$$

$$A\mathbf{b}_1 = \begin{pmatrix} 1 & 0 & 0 \\ 0 & 2 & 0 \\ 0 & 0 & 3 \end{pmatrix} \begin{pmatrix} 1 \\ 2 \\ 4 \end{pmatrix} = \begin{pmatrix} 1 \\ 4 \\ 12 \end{pmatrix}$$

Express in  $\mathcal{B}$ :

$$\begin{pmatrix} 1 \\ 4 \\ 12 \end{pmatrix} = c_1 \begin{pmatrix} 1 \\ 2 \\ 4 \end{pmatrix} + c_2 \begin{pmatrix} 0 \\ 1 \\ 0 \end{pmatrix} + c_3 \begin{pmatrix} 0 \\ 0 \\ 1 \end{pmatrix}$$

This gives  $c_1 = 1$ ,  $c_2 = 2$ ,  $c_3 = 8$ .

So,

$$[A\mathbf{b}_1]_{\mathcal{B}} = \begin{pmatrix} 1 \\ 2 \\ 8 \end{pmatrix}$$

$$A\mathbf{b}_2 = \begin{pmatrix} 1 & 0 & 0 \\ 0 & 2 & 0 \\ 0 & 0 & 3 \end{pmatrix} \begin{pmatrix} 0 \\ 1 \\ 0 \end{pmatrix} = \begin{pmatrix} 0 \\ 2 \\ 0 \end{pmatrix}$$

Express in  $\mathcal{B}$ :

$$\begin{pmatrix} 0 \\ 2 \\ 0 \end{pmatrix} = c_1 \begin{pmatrix} 1 \\ 2 \\ 4 \end{pmatrix} + c_2 \begin{pmatrix} 0 \\ 1 \\ 0 \end{pmatrix} + c_3 \begin{pmatrix} 0 \\ 0 \\ 1 \end{pmatrix}$$

This gives  $c_1 = 0$ ,  $c_2 = 2$ ,  $c_3 = 0$ . So,

$$[A\mathbf{b}_2]_{\mathcal{B}} = \begin{pmatrix} 0 \\ 2 \\ 0 \end{pmatrix}$$

$$A\mathbf{b}_3 = \begin{pmatrix} 1 & 0 & 0 \\ 0 & 2 & 0 \\ 0 & 0 & 3 \end{pmatrix} \begin{pmatrix} 0 \\ 0 \\ 1 \end{pmatrix} = \begin{pmatrix} 0 \\ 0 \\ 3 \end{pmatrix}$$

Express in  $\mathcal{B}$ :

$$\begin{pmatrix} 0 \\ 0 \\ 3 \end{pmatrix} = c_1 \begin{pmatrix} 1 \\ 2 \\ 4 \end{pmatrix} + c_2 \begin{pmatrix} 0 \\ 1 \\ 0 \end{pmatrix} + c_3 \begin{pmatrix} 0 \\ 0 \\ 1 \end{pmatrix}$$

This gives  $c_1 = 0$ ,  $c_2 = 0$ ,  $c_3 = 3$ . So,

$$[A\mathbf{b}_3]_{\mathcal{B}} = \begin{pmatrix} 0 \\ 0 \\ 3 \end{pmatrix}$$

The transformation matrix with respect to the basis  $\mathcal{B}$  is

$$[\varphi]_{\mathcal{B}} = \begin{pmatrix} 1 & 0 & 0 \\ 2 & 2 & 0 \\ 8 & 0 & 3 \end{pmatrix}.$$